Applied feedback from Cedric

examples/low-level/merkletree/merkle_tree.h
@@ -1,36 +1,15 @@
 // Interface
+// Assuming we have a `merkle_tree` structure
 
-typedef uint32_t hash_t;
+typedef uint8_t[32] hash_t;
+typedef uint8_t *path_t;
+typedef merkle_tree *mt_ptr;
 
-typedef struct extend_response_s
-{
-  uint32_t resp;
-  uint32_t idx; // do we need it?
-  hash_t root_signed;
-  hash_t[MAX_PATH_LENGTH] path;
-}
-  extend_response;
+mt_ptr create();
+void insert(mt_ptr mt, hash_t v);
+void get_root(mt_ptr mt, /*output*/ hash_t root);
 
-// For clients
-extend_response extend(data_t req);
-bool verify(data_t req, uint32_t resp, hash_t root, hash_t *path);
+// @param[idx]: an index of a (leaf) value in the tree
+// @return: the length of `path`
+uint32_t get_path(mt_ptr mt, uint32_t idx, /*output*/ path_t path);
 
-// For server (internally)
-// Interface extracted from KreMLin
-
-typedef struct merkle_tree_s
-{
-  uint32_t nelts;
-  elem *values;
-  hash *iroots;
-}
-  merkle_tree;
-
-merkle_tree create_merkle_tree();
-bool is_full(merkle_tree mt);
-merkle_tree insert(merkle_tree mt, data_t e);
-hash_t get_merkle_root(merkle_tree mt);
-  
-// Next-phase work
-
-hash_t *get_path(merkle_tree mt, uint32_t idx);
